Strata/Languages/Core/FactoryWF.lean
@@ -6,6 +6,7 @@
 
 import Strata.Languages.Core.Factory
 import Strata.DL.Lambda.Factory
+import Strata.DL.Util.Func
 import Strata.DL.Lambda.IntBoolFactory
 
 /-! # Factory Wellformedness Proof
@@ -36,10 +37,11 @@ theorem Factory_wf :
     intros Hmem
     repeat (
       rcases Hmem with _ | ⟨ a', Hmem ⟩
-      · apply LFuncWF.mk
+      · rw [LFuncWF]
+        apply Strata.DL.Util.FuncWF.mk
         · decide -- LFuncWF.arg_nodup
         · decide -- LFuncWF.body_freevars
-        · -- LFuncWf.concreteEval_argmatch
+        · -- LFuncWF.concreteEval_argmatch
           simp (config := { ground := true })
           try (
             try unfold unOpCeval
