Strata/Transform/CallElimCorrect.lean
@@ -183,6 +183,7 @@ theorem callElimBlockNoExcept :
   | ite cd tb eb md => exists [.ite cd tb eb md]
   | goto l b => exists [.goto l b]
   | loop g m i b md => exists [.loop g m i b md]
+  | funcDecl f md => exists [.funcDecl f md]
   | cmd c =>
     cases c with
     | cmd c' => exists [Imperative.Stmt.cmd (CmdExt.cmd c')]
@@ -617,9 +618,9 @@ theorem EvalStatementContractInitVar :
   Imperative.WellFormedSemanticEvalVar δ →
   σ v = some vv →
   σ v' = none →
-  EvalStatementContract π δ σ
+  EvalStatementContract π φ δ σ
     (createInitVar ((v', ty), v))
-    (updatedState σ v' vv) := by
+    (updatedState σ v' vv) δ := by
   intros Hwf Hsome Hnone
   simp [createInitVar]
   constructor
@@ -646,10 +647,10 @@ theorem EvalStatementsContractInitVars :
   List.Nodup ((trips.unzip.fst.unzip.fst) ++ (trips.unzip.snd)) →
   ReadValues σ (trips.unzip.snd) vvs →
   Imperative.isNotDefined σ (trips.unzip.fst.unzip.fst) →
-  EvalStatementsContract π δ σ
+  EvalStatementsContract π φ δ σ
     (createInitVars trips)
     (updatedStates σ
-      (trips.unzip.fst.unzip.fst) vvs) := by
+      (trips.unzip.fst.unzip.fst) vvs) δ := by
   intros Hwf Hndup Hdef Hndef
   induction trips generalizing σ vvs with
   | nil =>
@@ -687,9 +688,9 @@ theorem EvalStatementContractInit :
   Imperative.WellFormedSemanticEvalVar δ →
   δ σ e = some vv →
   σ v' = none →
-  EvalStatementContract π δ σ
+  EvalStatementContract π φ δ σ
     (createInit ((v', ty), e))
-    (updatedState σ v' vv) := by
+    (updatedState σ v' vv) δ := by
   intros Hwf Hsome Hnone
   simp [createInit]
   constructor
@@ -717,10 +718,10 @@ theorem EvalStatementsContractInits :
   EvalExpressions (P:=Core.Expression) δ σ (trips.unzip.2) vvs →
   -- ReadValues σ (trips.unzip.2) vvs →
   Imperative.isNotDefined σ (trips.unzip.1.unzip.1) →
-  EvalStatementsContract π δ σ
+  EvalStatementsContract π φ δ σ
     (createInits trips)
     (updatedStates σ
-      (trips.unzip.1.unzip.1) vvs) := by
+      (trips.unzip.1.unzip.1) vvs) δ := by
   intros Hwfvr Hwfvl Hwfc Hdisj Hndup Hdef Hndef
   induction trips generalizing σ vvs with
   | nil =>
@@ -758,9 +759,9 @@ theorem EvalStatementContractHavocUpdated :
   ∀ vv,
   Imperative.WellFormedSemanticEvalVar δ →
   σ v = some vv' →
-  EvalStatementContract π δ σ
+  EvalStatementContract π φ δ σ
     (createHavoc v)
-    (updatedState σ v vv) := by
+    (updatedState σ v vv) δ := by
   intros vv Hwf Hsome
   simp [createHavoc]
   constructor
@@ -846,8 +847,8 @@ theorem EvalStatementsContractHavocVars :
   Imperative.WellFormedSemanticEvalVar δ →
   Imperative.isDefined σ vs →
   HavocVars σ vs σ' →
-  EvalStatementsContract π δ σ
-    (createHavocs vs) σ' := by
+  EvalStatementsContract π φ δ σ
+    (createHavocs vs) σ' δ := by
   intros Hwfv Hdef Hhav
   simp [createHavocs]
   induction vs generalizing σ
@@ -1593,7 +1594,7 @@ theorem createAssertsCorrect :
   EvalExpressions δ σ (createFvars ks') vals →
   ReadValues σA ks vals →
   Imperative.substStores σ' σA (ks'.zip ks) →
-  EvalStatementsContract π δ σ' (createAsserts pres (ks.zip (createFvars ks'))) σ' := by
+  EvalStatementsContract π φ δ σ' (createAsserts pres (ks.zip (createFvars ks'))) σ' δ := by
    intros Hwfb Hwfvr Hwfvl Hwfc Hlen Hnd Hdef Hpres Heval Hrd Hsubst2
    simp [createAsserts]
    -- Make index parameter `i` explicit so that we can induct generalizing `i`.
@@ -1603,9 +1604,9 @@ theorem createAssertsCorrect :
          ((Imperative.HasVarsPure.getVars (P:=Expression) pre).removeAll (ks ++ ks')) ∧
        ks'.Disjoint (Imperative.HasVarsPure.getVars (P:=Expression) pre) ∧
        δ σA pre = some Imperative.HasBool.tt) →
-     EvalStatementsContract π δ σ'
+     EvalStatementsContract π φ δ σ'
        (List.mapIdx (fun j pred => Statement.assert s!"assert_{i + j}"
-         (Lambda.LExpr.substFvars pred (ks.zip (createFvars ks')))) l) σ'
+         (Lambda.LExpr.substFvars pred (ks.zip (createFvars ks')))) l) σ' δ
    by
     have := @h 0 pres Hpres
     simp at this; exact this
@@ -1649,7 +1650,7 @@ theorem createAssumesCorrect :
     ks'.Disjoint (Imperative.HasVarsPure.getVars (P:=Expression) post) ∧
     δ σA post = some Imperative.HasBool.tt) →
   Imperative.substStores σA σ' (ks.zip ks') →
-  EvalStatementsContract π δ σ' (createAssumes posts (ks.zip (createFvars ks'))) σ' := by
+  EvalStatementsContract π φ δ σ' (createAssumes posts (ks.zip (createFvars ks'))) σ' δ := by
    intros Hwfb Hwfvr Hwfvl Hwfc Hlen Hnd Hdef Hposts Hsubst2
    simp [createAssumes]
    -- Make index parameter `i` explicit so that we can induct generalizing `i`.
@@ -1659,9 +1660,9 @@ theorem createAssumesCorrect :
          ((Imperative.HasVarsPure.getVars (P:=Expression) post).removeAll (ks ++ ks')) ∧
        ks'.Disjoint (Imperative.HasVarsPure.getVars (P:=Expression) post) ∧
        δ σA post = some Imperative.HasBool.tt) →
-     EvalStatementsContract π δ σ'
+     EvalStatementsContract π φ δ σ'
        (List.mapIdx (fun j pred => Statement.assume s!"assume_{i + j}"
-         (Lambda.LExpr.substFvars pred (ks.zip (createFvars ks')))) l) σ'
+         (Lambda.LExpr.substFvars pred (ks.zip (createFvars ks')))) l) σ' δ
    by
     have := @h 0 posts Hposts
     simp at this; exact this
@@ -3285,7 +3286,7 @@ theorem callElimStatementCorrect [LawfulBEq Expression.Expr] :
   (∀ pname, π pname = (Program.Procedure.find? p (.unres pname))) →
   -- all global variables in p exist in σ
   (∀ gk, (p.find? .var gk).isSome → (σ gk).isSome) →
-  EvalStatementsContract π δ σ [st] σ' →
+  EvalStatementsContract π φ δ σ [st] σ' δ →
   WellFormedCoreEvalCong δ →
   WF.WFStatementsProp p [st] →
   WF.WFProgramProp p →
@@ -3295,7 +3296,7 @@ theorem callElimStatementCorrect [LawfulBEq Expression.Expr] :
   -- NOTE: The theorem does not expect the same store due to inserting new temp variables
   exists σ'',
     Inits σ' σ'' ∧
-    EvalStatementsContract π δ σ sts σ''
+    EvalStatementsContract π φ δ σ sts σ'' δ
     := by
   intros Hp Hgv Heval Hwfc Hwf Hwfp Hwfgen Hwfgenst Helim
   cases st <;>
@@ -3308,6 +3309,7 @@ theorem callElimStatementCorrect [LawfulBEq Expression.Expr] :
   case ite => exact ⟨σ', Inits.init InitVars.init_none, Heval⟩
   case goto => exact ⟨σ', Inits.init InitVars.init_none, Heval⟩
   case loop => exact ⟨σ', Inits.init InitVars.init_none, Heval⟩
+  case funcDecl => exact ⟨σ', Inits.init InitVars.init_none, Heval⟩
   case cmd c =>
   cases c with
   | cmd c' =>
@@ -3457,7 +3459,8 @@ theorem callElimStatementCorrect [LawfulBEq Expression.Expr] :
                       (argTrips.unzip.fst.unzip.fst ++
                       outTrips.unzip.fst.unzip.fst ++
                       oldTrips.unzip.fst.unzip.fst) := by
-        simp only [EvalBlockEmpty Heval2] at *
+        have ⟨Hσeq, _⟩ := Imperative.EvalBlockEmpty Heval2
+        simp only [← Hσeq]
         apply UpdateStatesNotDefMonotone ?_ Hupdate
         intros v Hin
         have Htemp : v.isTemp = true := by
